More cleanup: separate AST for convenience in typing judgements.

SkLean/Ast.lean
@@ -1,6 +1,8 @@
 /-
 # AST
 
+## SK Dependent Typing
+
 I interpret the SK combinators as dependently typed functions of the form:
 
 $$
@@ -14,12 +16,13 @@ Borrowing from the calculus of constructions, the types of \\(K\\) and \\(S\\) a
 
 $$
 K : (\forall \alpha : \text{Type}\ m, \beta : \text{Type}\ n, x : \alpha\ y : \beta . \alpha) \\\\
-S : (\forall \alpha : \text{Type}\ m, \beta : \text{Type}\ n, \gamma : \text{Type}\ o, x : (\forall x : \alpha, y : \beta, z : \gamma . \gamma), y : (\forall x : \alpha, y : \beta . \alpha), z : \alpha . \gamma)
+S : (\forall \alpha : \text{Type}\ m, \beta : \text{Type}\ n, \gamma : \text{Type}\ o, \\\\
+x : (\forall x : \alpha, y : \beta, z : \gamma . \gamma), y : (\forall x : \alpha . \beta), z : \alpha . \gamma)
 $$
 
 Typing judgements on function application are derived from substitution on \\(\forall\\). For example, the type of \\(K\ \mathbb{N}\\) is derived from substitution of \\(\mathbb{N}\\) into the type of \\(K\\). That is, \\(\alpha\\) is replaced with \\(\mathbb{N}\\), and the type of the expression is said to be equal to the body of the \\(\forall\\) in which the value was substituted.
 
-The K and S combinators can be encoded in AST form in Lean using De Bruijn indices like such:
+The \\(K\\) and \\(S\\) combinators can be encoded in AST form in Lean using De Bruijn indices like such:
 -/
 
 import Mathlib.Tactic
@@ -29,7 +32,7 @@ A `BindId n` refers to the value of the variable binder in the nth-up \\(\forall
 -/
 structure BindId where
   toNat : ℕ
-deriving BEq, Repr
+deriving BEq, Repr, DecidableEq
 
 namespace BindId
 
@@ -48,17 +51,64 @@ end BindId
 For example, the expression \\(\forall x : \alpha.x\\) can be rewritten using De Bruijn indices to \\(\forall \alpha.1\\).
 
 An expression is one of: \\(K\\), \\(S\\), \\(\text{Prop}\\), \\(\text{Ty}\ n\\), \\((\forall e_{1}.e_{2})\\), \\(e_{1}\ e_{2}\\), or a variable \\(n\\).
+
+For convenience and legibility, I create a separate definition of each expression:
 -/
 
+mutual
+
+inductive K where
+  | mk : K
+
+inductive S where
+  | mk : S
+
+inductive Prp where
+  | mk : Prp
+
+/-
+Stratified type universes.
+-/
+inductive Ty where
+  | mk : ℕ → Ty
+
+inductive Call where
+  | mk : SkExpr → SkExpr → Call
+
+/-
+Var uses a 1-indexed De Bruijn position.
+-/
+
+inductive Var where
+  | mk : BindId → Var
+
+/-
+\\(\forall\\) takes a type of its binder \\(x : t\\), and has a body containing \\(e\\).
+-/
+inductive Fall where
+  | mk : SkExpr → SkExpr → Fall
+
 inductive SkExpr where
-  | k    : SkExpr
-  | s    : SkExpr
-  | prp  : SkExpr
-  | ty   : ℕ      → SkExpr
-  | fall : SkExpr → SkExpr → SkExpr
-  | call : SkExpr → SkExpr → SkExpr
-  | var  : BindId → SkExpr
+  | k    : K    → SkExpr
+  | s    : S    → SkExpr
+  | prp  : Prp  → SkExpr
+  | ty   : Ty   → SkExpr
+  | fall : Fall → SkExpr
+  | call : Call → SkExpr
+  | var  : Var  → SkExpr
 deriving BEq, Repr
+
+end
+
+namespace Call
+
+def lhs : Call → SkExpr
+  | .mk lhs _ => lhs
+
+def rhs : Call → SkExpr
+  | .mk _ rhs => rhs
+
+end Call
 
 namespace SkExpr
 
@@ -68,87 +118,83 @@ Whenever a value is substituted in to a \\(\forall\\) expression, all its free v
 
 def with_indices_plus (in_expr : SkExpr) (shift_by : BindId) : SkExpr :=
   match in_expr with
-    | fall bind_ty body =>
-      fall (bind_ty.with_indices_plus shift_by.succ) (body.with_indices_plus shift_by.succ)
-    | var n =>
+    | .fall (.mk bind_ty body) =>
+      .fall (.mk (bind_ty.with_indices_plus shift_by.succ) (body.with_indices_plus shift_by.succ))
+    | .var (.mk n) =>
       if n > shift_by then
-        var ⟨n.toNat + shift_by.toNat⟩
+        var (.mk ⟨n.toNat + shift_by.toNat⟩)
       else
-        var n
-    | call lhs rhs =>
-      call (lhs.with_indices_plus shift_by) (rhs.with_indices_plus shift_by)
+        var (.mk n)
+    | .call (.mk lhs rhs) =>
+      call (.mk (lhs.with_indices_plus shift_by) (rhs.with_indices_plus shift_by))
     | x => x
 
-def substitute (in_expr : SkExpr) (n : BindId) (with_expr : SkExpr) : SkExpr :=
-  match in_expr with
-    | fall bind_ty body =>
-      fall (bind_ty.substitute n.succ with_expr) (body.substitute n.succ with_expr)
-    | var n' => if n == n' then with_expr.with_indices_plus n else var n'
-    | x => x
+end SkExpr
+
+namespace Fall
+
+def body : Fall → SkExpr
+  | .mk _ body => body
+
+def substitute (in_fall : Fall) (with_expr : SkExpr) : Fall :=
+  let rec substitute_e (in_expr : SkExpr) (n : BindId) (with_expr : SkExpr) : SkExpr :=
+    match in_expr with
+      | .fall (.mk bind_ty body) =>
+        .fall (.mk (substitute_e bind_ty n.succ with_expr) (substitute_e body n.succ with_expr))
+      | .var (.mk n') => if n = n' then with_expr.with_indices_plus n else .var (.mk n')
+      | x => x
+    match in_fall with
+      | .mk bind_ty body =>
+        .mk (substitute_e bind_ty ⟨1⟩ with_expr) (substitute_e body ⟨1⟩ with_expr)
+
+end Fall
 
 /-
 I give a few test cases of index shifting:
 -/
 
-example : (fall (ty 0) (var ⟨2⟩)).with_indices_plus ⟨1⟩ = (fall (ty 0) (var ⟨2⟩)) := by
-  repeat unfold with_indices_plus
-  simp
-  intro h
-  unfold BindId.succ
-  simp
-  contradiction
-
-example : (fall (ty 0) (var ⟨1⟩)).substitute ⟨0⟩ (var ⟨2⟩) = (fall (ty 0) (var ⟨3⟩)) := by
-  unfold substitute
-  simp
-  repeat unfold substitute
-  simp
-  split
-  repeat unfold with_indices_plus
-  simp
-  split
+example : (SkExpr.fall (.mk (.ty (.mk 0)) (.var (.mk ⟨2⟩)))).with_indices_plus ⟨1⟩ = (SkExpr.fall (.mk (.ty (.mk 0)) (.var (.mk ⟨2⟩)))) := by
+  repeat unfold SkExpr.with_indices_plus
   simp
   unfold BindId.succ
   simp
-  contradiction
-  simp_all
-  repeat unfold BindId.succ at *
-  simp_all
-  contradiction
-
-example : (fall (ty 0) (var ⟨1⟩)).substitute ⟨0⟩ (fall (ty 0) (var ⟨4⟩)) = (fall (ty 0) ((fall (ty 0) (var ⟨6⟩)))) := by
-  unfold substitute
+  unfold LT.lt
+  unfold BindId.instLT
   simp
-  repeat unfold substitute
+
+example : ((Fall.mk (.ty (.mk 0)) (.var (.mk ⟨1⟩)))).substitute (.var (.mk ⟨2⟩)) = (Fall.mk (.ty (.mk 0)) (.var (.mk ⟨3⟩))) := by
+  unfold Fall.substitute
+  simp
+  repeat unfold Fall.substitute.substitute_e
+  simp
+  repeat unfold SkExpr.with_indices_plus
+  simp
+  unfold LT.lt
+  unfold BindId.instLT
+  simp
+
+example : (Fall.mk (.ty (.mk 0)) (.var (.mk ⟨1⟩))).substitute (.fall (.mk (.ty (.mk 0)) (.var (.mk ⟨4⟩)))) = (Fall.mk (.ty (.mk 0)) ((.fall (.mk (.ty (.mk 0)) (.var (.mk ⟨6⟩)))))) := by
+  unfold Fall.substitute
+  simp
+  repeat unfold Fall.substitute.substitute_e
+  simp
+  repeat unfold SkExpr.with_indices_plus
   simp
   split
-  case isTrue h =>
-    repeat unfold with_indices_plus
-    simp
-    repeat unfold BindId.succ at *
-    simp_all
-    unfold LT.lt
-    unfold BindId.instLT
-    simp
-  case isFalse h =>
-    simp_all
-    contradiction
-
-/-
-When inferring the type of a function application, the rhs of the application is substituted in to the left hand side's type (\\(\forall\\)). The type of the application is said to be equivalent to the body of the substituted \\(\forall\\). See [type inference rules](./Typing.lean.md) for more.
--/
-
-def body : SkExpr → Option SkExpr
-  | fall _ body => some body
-  | _ => none
+  simp
+  repeat unfold BindId.succ
+  simp
+  contradiction
 
 /-
 One-step evaluation is only defined for \\(K\ \alpha\ \beta\ x\ y\\) and \\(S\ \alpha\ \beta\ \gamma\ x\ y\ z\\).
 -/
 
-def eval_once : SkExpr → SkExpr
-  | (call (call (call (call k _) _) x) _) => x
-  | call (call (call (call (call (call s _) _) _) x) y) z => call (call x z) (call y z)
-  | x => x
+namespace SkExpr
+
+def eval_once : Call → SkExpr
+  | (.mk (.call (.mk (.call (.mk (.call (.mk (.call (.mk (.k .mk) _)) _)) _)) x)) _) => x
+  | (.mk (.call (.mk (.call (.mk (.call (.mk (.call (.mk (.call (.mk (.s .mk)  _)) _)) _)) x)) y)) z) => .call (.mk (.call (.mk x z)) (.call (.mk y z)))
+  | (.mk x y) => (.call (.mk x y))
 
 end SkExpr
